test/Mutable/thunk1.lean
@@ -12,7 +12,7 @@ protected def Thunk'.pure (a : α) : Thunk' α :=
   .mk fun _ ↦ a
 
 protected def Thunk'.get (x : Thunk' α) : α :=
-  Mutable.getModify₂ x (fun f ↦ let a := f (); ⟨a, fun _ ↦ a⟩) (fun _ ↦ rfl)
+  Mutable.getModify x (fun f ↦ let a := f (); ⟨a, fun _ ↦ a⟩) (fun _ ↦ rfl)
 
 @[inline] protected def Thunk'.map (f : α → β) (x : Thunk' α) : Thunk' β :=
   .mk fun _ => f x.get
@@ -23,46 +23,43 @@ protected def Thunk'.get (x : Thunk' α) : α :=
 /-! lean4/tests/lean/thunk.lean -/
 
 /-- info: 1 -/
-#guard_msgs in #eval
-  (Thunk'.pure 1).get
+#guard_msgs in #eval (Thunk'.pure 1).get
 /-- info: 2 -/
 #guard_msgs in #eval (Thunk'.mk fun _ => 2).get
 /--
 info: 3
 4
-5
+---
+info: 5
 -/
 #guard_msgs in #eval
   let t1 := Thunk'.mk fun _ => dbg_trace 4; 5
-  -- let t2 := Thunk'.mk fun _ => dbg_trace 3; 0
-  -- let v2 := t2.get
-  let v2 := dbg_trace 3; 0
-
+  let t2 := Thunk'.mk fun _ => dbg_trace 3; 0
+  let v2 := t2.get
   let v1 := t1.get
   v1 + v2
 /--
 info: 6
 7
-8
+---
+info: 8
 -/
 #guard_msgs in #eval
   let t1 := Thunk'.pure 8 |>.map fun n => dbg_trace 7; n
-  -- let t2 := Thunk'.mk fun _ => dbg_trace 6; 0
-  -- let v2 := t2.get
-  let v2 := dbg_trace 6; 0
-
+  let t2 := Thunk'.mk fun _ => dbg_trace 6; 0
+  let v2 := t2.get
   let v1 := t1.get
   v1 + v2
+
 /--
 info: 9
 10
-11
+---
+info: 11
 -/
 #guard_msgs in #eval
   let t1 := Thunk'.pure 11 |>.bind fun n => dbg_trace 10; Thunk'.pure n
-  -- let t2 := Thunk'.mk fun _ => dbg_trace 9; 0
-  -- let v2 := t2.get
-  let v2 := dbg_trace 9; 0
-
+  let t2 := Thunk'.mk fun _ => dbg_trace 9; 0
+  let v2 := t2.get
   let v1 := t1.get
   v1 + v2
